Cleanup and documentation of entire alpha equivalence framework

src/Language/STLC/Alpha/alpha_kinding.v
@@ -5,69 +5,63 @@ From PlutusCert Require Import variables util Alpha.alpha STLC STLC.Kinding Util
 Local Open Scope string_scope.
 Local Open Scope list_scope.
 
-(* Alpha equivalence of types *)
-
-(* Contextual alpha equivalence: kinding contexts that match alpha contexts*)
+(* Alpha equivalence of kinding contexts *)
 Inductive CAlpha : list (string * string) -> list (string * PlutusIR.kind) -> list (string * PlutusIR.kind) -> Prop :=
-  | calpha_nil D : CAlpha [] D D (* Non-empty kinding enviornments because id renamings are like no renamings. TODO: think whether we want to allow that or want to enforce that id renamings are in the alpha enviornment always*)
-  | calpha_cons x y K sigma Gamma Gamma' :
-    CAlpha sigma Gamma Gamma' ->
-    CAlpha ((x, y)::sigma) ((x, K)::Gamma) ((y, K)::Gamma').
-  (* | calpha_id x K sigma Gamma Gamma' :
-    CAlpha sigma Gamma Gamma' ->
-    CAlpha sigma ((x, K)::Gamma) ((x, K)::Gamma'). *)
+  | calpha_nil D : CAlpha [] D D 
+  | calpha_cons x y K R Γ Γ' :
+    CAlpha R Γ Γ' ->
+    CAlpha ((x, y)::R) ((x, K)::Γ) ((y, K)::Γ').
 
 Set Printing Implicit.
 
-(* Exercise and possibly useful *)
-Lemma alpha_preserves_kinding sigma s t A Gamma Gamma' :
-  Alpha sigma s t -> CAlpha sigma Gamma Gamma' -> STLC.Kinding.has_kind Gamma s A -> STLC.Kinding.has_kind Gamma' t A.
+(* Well-kindedness is preserved under alpha equivalence *)
+Lemma alpha_preserves_kinding R s t A Γ Γ' :
+  Alpha R s t -> CAlpha R Γ Γ' -> STLC.Kinding.has_kind Γ s A -> STLC.Kinding.has_kind Γ' t A.
 Proof.
   intros HAlpha Htype.
   generalize dependent A.
-  generalize dependent Gamma.
-  generalize dependent Gamma'.
+  generalize dependent Γ.
+  generalize dependent Γ'.
   induction HAlpha.
-  - intros Gamma' Gamma HCAlpha A HType.
+  - intros Γ' Γ HCAlpha A HType.
     inversion HType.
     apply K_Var; subst...
-    generalize dependent Gamma.
-    generalize dependent Gamma'.
+    generalize dependent Γ.
+    generalize dependent Γ'.
     induction a; subst...
     + intros.
       inversion HCAlpha; subst...
       assumption.
-    + intros Gamma' Gamma HCAlpha HType Hlookup.
+    + intros Γ' Γ HCAlpha HType Hlookup.
       inversion HCAlpha; subst...
       inversion Hlookup.
       simpl.
       repeat rewrite Coq.Strings.String.eqb_refl.
       reflexivity.
-    + intros Gamma' Gamma HCAlpha HType Hlookup.
+    + intros Γ' Γ HCAlpha HType Hlookup.
       inversion HCAlpha; subst...
       simpl.
       destruct (y =? w) eqn:yw.
       * apply String.eqb_eq in yw.
         contradiction.
-      * specialize (IHa Gamma'0 Gamma0 H4).
+      * specialize (IHa Γ'0 Γ0 H4).
         unfold lookup in Hlookup.
         destruct (x =? z) eqn:xz.
         -- apply String.eqb_eq in xz.
            contradiction.
-        -- fold (lookup z Gamma0) in Hlookup.
-          assert (Gamma0 |-* (tmvar z) : A).
+        -- fold (lookup z Γ0) in Hlookup.
+          assert (Γ0 |-* (tmvar z) : A).
           {
-            (* Strengthening typing*)
             apply K_Var.
             assumption.
           }
            specialize (IHa H Hlookup).
            assumption.
-  - intros Gamma' Gamma HCAlpha A0 HType.
+  - intros Γ' Γ HCAlpha A0 HType.
     inversion HType; subst;
-    specialize (IHHAlpha ((y, A)::Gamma') ((x, A)::Gamma)
-      (calpha_cons x y A R Gamma Gamma' HCAlpha) _ H5); constructor; auto.
-  - intros Gamma' Gamma HCAlpha A HType. 
+    specialize (IHHAlpha ((y, A)::Γ') ((x, A)::Γ)
+      (calpha_cons x y A R Γ Γ' HCAlpha) _ H5); constructor; auto.
+  - intros Γ' Γ HCAlpha A HType. 
     inversion HType; subst; econstructor; eauto.
   - intros.
     inversion H; subst.
