src/Language/STLC/Alpha/alpha_subs.v
@@ -6,17 +6,17 @@ Require Import Coq.Program.Equality.
 Require Import ssreflect.
 
 (* One subsitution is related to the other through the alpha context*)
-Inductive alphaSubs : list (string * string) -> list (string * term) -> list (string * term) -> Set :=
-  | alpha_ctx_nil R : alphaSubs R [] []
-  | alpha_ctx_cons R σ σ' x y t t' :
-    alphaSubs R σ σ' ->
+Inductive AlphaSubs : list (string * string) -> list (string * term) -> list (string * term) -> Set :=
+  | AlphaSubs_nil R : AlphaSubs R [] []
+  | AlphaSubs_cons R σ σ' x y t t' :
+    AlphaSubs R σ σ' ->
     AlphaVar R x y ->
     Alpha R t t' ->
-    alphaSubs R ((x, t)::σ) ((y, t')::σ').
+    AlphaSubs R ((x, t)::σ) ((y, t')::σ').
 
-
-Lemma αctx_sym σ σ' R :
-  alphaSubs R σ σ' -> alphaSubs (sym_alpha_ctx R) σ' σ.
+(* Symmetry of α-equivalent substitutions*)
+Lemma AlphaSubs_sym σ σ' R :
+  AlphaSubs R σ σ' -> AlphaSubs (sym_alpha_ctx R) σ' σ.
 Proof.
   intros Hctx.
   induction Hctx.
@@ -25,8 +25,9 @@ Proof.
   - eapply alpha_sym; eauto. apply sym_alpha_ctx_is_sym.
 Qed.
 
-Lemma alpha_ctx_right_ex {R sigma sigma' x x' t }:
-  alphaSubs R sigma sigma' ->
+(* Existence of variables in a substitution σ implies existence in σ': right *)
+Lemma AlphaSubs_right_ex {R sigma sigma' x x' t }:
+  AlphaSubs R sigma sigma' ->
   AlphaVar R x x' ->
   lookup x sigma = Some t ->
   {t' & prod (lookup x' sigma' = Some t') (Alpha R t t')}.
@@ -41,13 +42,14 @@ Proof.
   - remember H0 as Hav_xx'; clear HeqHav_xx'.
     apply (alphavar_unique_not_left H2 a) in H0.
     simpl in H1. rewrite <- String.eqb_neq in H2. rewrite H2 in H1.
-    specialize (IHalphaSubs Hav_xx' H1) as [t'0 [Hlookup Ha_t]].
+    specialize (IHAlphaSubs Hav_xx' H1) as [t'0 [Hlookup Ha_t]].
     exists t'0. split; auto.
     simpl. rewrite <- String.eqb_neq in H0. rewrite H0. auto.
 Qed.
 
-Lemma alpha_ctx_left_ex {R sigma sigma' x x' t' }:
-  alphaSubs R sigma sigma' ->
+(* Existence of variables in a substitution σ implies existence in σ': left *)
+Lemma AlphaSubs_left_ex {R sigma sigma' x x' t' }:
+  AlphaSubs R sigma sigma' ->
   AlphaVar R x x' ->
   lookup x' sigma' = Some t' ->
   { t & prod (lookup x sigma = Some t) (Alpha R t t')}.
@@ -55,15 +57,16 @@ Proof.
   intros Hctx HA_x Hl.
   eapply @alphavar_sym with (R' := sym_alpha_ctx R) in HA_x; auto.
   2: { apply sym_alpha_ctx_is_sym. }
-  apply @αctx_sym with (R := R) in Hctx; auto.
-  eapply alpha_ctx_right_ex in Hl as [t'' [Hl_t'' Ha_t']]; eauto.
+  apply @AlphaSubs_sym with (R := R) in Hctx; auto.
+  eapply AlphaSubs_right_ex in Hl as [t'' [Hl_t'' Ha_t']]; eauto.
   exists t''. split; auto.
   eapply @alpha_sym with (R := (sym_alpha_ctx R)); auto.
   apply sym_alpha_ctx_left_is_sym.
 Qed.
 
-Lemma alpha_ctx_left_nex {R sigma sigma' x x'}:
-  alphaSubs R sigma sigma' ->
+(* Inexistence of variables in a substitution σ implies inexistence in σ': left *)
+Lemma AlphaSubs_left_nex {R sigma sigma' x x'}:
+  AlphaSubs R sigma sigma' ->
   AlphaVar R x x' ->
   lookup x' sigma' = None ->
   lookup x sigma = None.
@@ -74,12 +77,13 @@ Proof.
   apply in_map_iff in Hcontra as [ [x'' t] [Hlookup Hcontra'] ].
   apply in_map__exists_lookup in Hcontra' as [t' Hl_t'].
   simpl in Hlookup. subst.
-  eapply (alpha_ctx_right_ex Hctx HA_x) in Hl_t' as [t'0 [Hl_t'0 Ha_t'0]].
+  eapply (AlphaSubs_right_ex Hctx HA_x) in Hl_t' as [t'0 [Hl_t'0 Ha_t'0]].
   congruence.
 Qed.
 
-Lemma alpha_ctx_right_nex {R sigma sigma' x x'}:
-  alphaSubs R sigma sigma' ->
+(* Inexistence of variables in a substitution σ implies inexistence in σ': right *)
+Lemma AlphaSubs_right_nex {R sigma sigma' x x'}:
+  AlphaSubs R sigma sigma' ->
   AlphaVar R x x' ->
   lookup x sigma = None ->
   lookup x' sigma' = None.
@@ -90,24 +94,26 @@ Proof.
   apply in_map_iff in Hcontra as [ [x'' t] [Hlookup Hcontra'] ].
   apply in_map__exists_lookup in Hcontra' as [t' Hl_t'].
   simpl in Hlookup. subst.
-  eapply (alpha_ctx_left_ex Hctx HA_x) in Hl_t' as [t'0 [Hl_t'0 Ha_t'0]].
+  eapply (AlphaSubs_left_ex Hctx HA_x) in Hl_t' as [t'0 [Hl_t'0 Ha_t'0]].
   congruence.
 Qed.
 
-Lemma alpha_ctx_R_nil {sigma }:
-  alphaSubs [] sigma sigma.
+(* Syntactically identical substitutions are α-equivalent in an empty renaming context*)
+Lemma AlphaSubs_R_nil {sigma }:
+  AlphaSubs [] sigma sigma.
 Proof.
   induction sigma.
-  - apply alpha_ctx_nil.
+  - apply AlphaSubs_nil.
   - destruct a.
-    apply alpha_ctx_cons; auto.
+    apply AlphaSubs_cons; auto.
     + apply alpha_var_refl.
     + apply alpha_refl. apply id_ctx_nil.
 Qed.
 
-Lemma αctx_trans R1 R2 R σ σ' σ'' :
+(* Transitivity of α-equivalent substitutions*)
+Lemma AlphaSubs_trans R1 R2 R σ σ' σ'' :
   αCtxTrans R1 R2 R -> 
-  alphaSubs R1 σ σ' -> alphaSubs R2 σ' σ'' -> alphaSubs R σ σ''.
+  AlphaSubs R1 σ σ' -> AlphaSubs R2 σ' σ'' -> AlphaSubs R σ σ''.
 Proof.
   intros.
   dependent induction σ.
@@ -122,8 +128,9 @@ Proof.
     + eapply alpha_trans; eauto.
 Qed.
 
-Lemma αctx_sub_extend_ids_right σ σ' R1 R2 :
-  IdCtx R2 -> alphaSubs R1 σ σ' -> alphaSubs (R1 ++ R2) σ σ'.
+(* Extension of identiy renamings on the right of an existing context is always allowed*)
+Lemma AlphaSubs_sub_extend_ids_right σ σ' R1 R2 :
+  IdCtx R2 -> AlphaSubs R1 σ σ' -> AlphaSubs (R1 ++ R2) σ σ'.
 Proof.
   intros HidR2 Ha.
   dependent induction σ.
