src/Language/STLC/Alpha/alpha_rename.v
@@ -10,19 +10,17 @@ Local Open Scope list_scope.
 *)
 
 (* We use bound and free because it is easier to reason about.
- e.g. x not free in any subterm of \x. y
- But it is bound in there.
-  while in \x.x it is free in the subterm.
-If we just take bound terms always as well, I think it is easier to reason.
+    e.g. x not free in any subterm of \x. y
+    But it is bound in there.
+      while in \x.x it is free in the subterm.
 
 Also, we need a freshness condition since renaming is not capture-avoiding.
 
 Correspondence between alpha contexts and renamings on syntactically equal terms.
  *)
-Lemma alphaRename x x' s :
-  (* x' can be equal to x., but then x=x' not in s, so the renaming doesnt do anything. 
-    Cannot easily be restricted to ftv: say s = λ x' . x. Then x' not free in s, but rename x x' s, will cause capture
-  *)
+(* Note: x' can be equal to x., but then x=x' not in s, so the renaming doesnt do anything.  *)
+(* Note: Cannot be restricted to only ftv: say s = λ x' . x. Then x' not free in s, but rename x x' s, will cause capture *)
+Lemma alpha_rename x x' s :
   ~ (In x' (tv s)) -> Alpha [(x, x')] s (rename x x' s).
 Proof.
   intros Hfresh.
@@ -107,10 +105,9 @@ Qed.
 
 
 (*
- Stronger result where s and s' not syntactically equal
-  New idea! Finally work with high-level ideas instead of induction on terms!
+  Strengthened renaming lemma for alpha-equivalent terms (rather than syntactically equal terms like above).
 *)
-Lemma alphaRenameStronger x x' s s' R :
+Lemma alpha_rename' x x' s s' R :
   ~ (In x' (tv s')) -> 
   NotBreakShadowing x R ->
   Alpha R s s' -> Alpha ((x, x')::R) s (rename x x' s').
@@ -122,9 +119,19 @@ Proof.
   - apply alpha_extend_id; eauto.
   - apply alpha_extend_ids_right with (R := (x, x')::nil).
     + apply ctx_id_right_is_id.
-    + now apply alphaRename.
+    + now apply alpha_rename.
 Qed.
 
+(*****
+  alpha_trans_rename_left and alpha_trans_rename_right
+  If we reach v from u by renaming s into s''
+  Then we can rename s'' and reflect that both in the term and the renaming context.
+*)
+(*
+  Used in the lambda abstraction inductive case of proofs dealing with capture-avoiding substitutions:
+  We know λs.u ~ λs''.v. Then because of capture, s'' gets renamed to b''.
+  Then we still have λs.u ~ λb''.rename s'' b'' v.
+ *)
 Lemma alpha_trans_rename_right u v b'' s'' s R sigma :
   b'' = fresh2 sigma v ->
   Alpha ((s, s'')::R) u v ->
@@ -134,7 +141,7 @@ Proof.
   eapply @alpha_trans with (R1 := ((s'', b'')::nil) ++ (ctx_id_right R)); eauto.
   - apply alpha_trans_cons. apply id_right_trans.
   - apply alpha_extend_ids_right; [apply ctx_id_right_is_id |].
-    apply alphaRename.
+    apply alpha_rename.
     now apply fresh2_over_tv_term in H.
 Qed.
 
@@ -148,6 +155,6 @@ Proof.
   - apply alpha_trans_cons. apply id_left_trans.
   - apply alpha_extend_ids_right; [apply ctx_id_left_is_id |].
     eapply alpha_sym; [repeat constructor|].
-    apply alphaRename.
+    apply alpha_rename.
     now apply fresh2_over_tv_term in H.
 Qed.
